all rules checking in CakeML

cakeml/fitchProgScript.sml
@@ -7,11 +7,7 @@ val _ = new_theory "fitchProg";
 
 val _ = translation_extends "MapProg";
 
-val _ = ml_prog_update (open_module "fitchProg");
-
-val _ = ml_prog_update open_local_block;
-
-(*val res = translate MEMBER_def;*)
+val _ = ml_prog_update (open_module "FitchProg");
 
 Definition valid_derivation_deriv_premise_cake:
  valid_derivation_deriv_premise_cake pl p = MEMBER p pl
@@ -60,6 +56,375 @@ QED
 
 val res = translate valid_derivation_deriv_copy_cake;
 
+Definition valid_derivation_deriv_andi_cake:
+ valid_derivation_deriv_andi_cake t l1 l2 p =
+   case lookup t (INL l1) of
+   | SOME (INL p1) =>
+     (case lookup t (INL l2) of
+     | SOME (INL p2) => p = prop_and p1 p2
+     | _ => F)
+   | _ => F
+End
+
+Theorem valid_derivation_deriv_andi_eq:
+ !t l1 l2 p. map_ok t ==>
+  valid_derivation_deriv_andi_cake t l1 l2 p = 
+   valid_derivation_deriv_andi (to_fmap t) l1 l2 p
+Proof
+ rw [valid_derivation_deriv_andi_cake,valid_derivation_deriv_andi] \\
+ rw [lookup_thm]
+QED
+
+val res = translate valid_derivation_deriv_andi_cake;
+
+Definition valid_derivation_deriv_ande1_cake:
+ valid_derivation_deriv_ande1_cake t l p =
+   case lookup t (INL l) of
+   | SOME (INL (prop_and p1 p2)) => p = p1
+   | _ => F
+End
+
+Theorem valid_derivation_deriv_ande1_eq:
+ !t l p. map_ok t ==>
+  valid_derivation_deriv_ande1_cake t l p = 
+   valid_derivation_deriv_ande1 (to_fmap t) l p
+Proof
+ rw [valid_derivation_deriv_ande1_cake,valid_derivation_deriv_ande1] \\
+ rw [lookup_thm]
+QED
+
+val res = translate valid_derivation_deriv_ande1_cake;
+
+Definition valid_derivation_deriv_ande2_cake:
+ valid_derivation_deriv_ande2_cake t l p =
+   case lookup t (INL l) of
+   | SOME (INL (prop_and p1 p2)) => p = p2
+   | _ => F
+End
+
+Theorem valid_derivation_deriv_ande2_eq:
+ !t l p. map_ok t ==>
+  valid_derivation_deriv_ande2_cake t l p = 
+   valid_derivation_deriv_ande2 (to_fmap t) l p
+Proof
+ rw [valid_derivation_deriv_ande2_cake,valid_derivation_deriv_ande2] \\
+ rw [lookup_thm]
+QED
+
+val res = translate valid_derivation_deriv_ande2_cake;
+
+Definition valid_derivation_deriv_ori1_cake:
+ valid_derivation_deriv_ori1_cake t l p =
+  case p of
+  | prop_or p1 p2 =>
+    (case lookup t (INL l) of
+     | SOME (INL p') => p1 = p'
+     | _ => F)
+  | _ => F
+End
+
+Theorem valid_derivation_deriv_ori1_eq:
+ !t l p. map_ok t ==>
+  valid_derivation_deriv_ori1_cake t l p = 
+   valid_derivation_deriv_ori1 (to_fmap t) l p
+Proof
+ rw [valid_derivation_deriv_ori1_cake,valid_derivation_deriv_ori1] \\
+ rw [lookup_thm]
+QED
+
+val res = translate valid_derivation_deriv_ori1_cake;
+
+Definition valid_derivation_deriv_ori2_cake:
+ valid_derivation_deriv_ori2_cake t l p =
+   case p of
+   | prop_or p1 p2 => 
+     (case lookup t (INL l) of
+       | SOME (INL p') => p2 = p'	 
+       | _ => F)
+   | _ => F
+End
+
+Theorem valid_derivation_deriv_ori2_eq:
+ !t l p. map_ok t ==>
+  valid_derivation_deriv_ori2_cake t l p = 
+   valid_derivation_deriv_ori2 (to_fmap t) l p
+Proof
+ rw [valid_derivation_deriv_ori2_cake,valid_derivation_deriv_ori2] \\
+ rw [lookup_thm]
+QED
+
+val res = translate valid_derivation_deriv_ori2_cake;
+
+Definition valid_derivation_deriv_impe_cake:
+ valid_derivation_deriv_impe_cake t l1 l2 p =
+   case lookup t (INL l1) of
+   | SOME (INL p1) => 
+     (case lookup t (INL l2) of
+      | SOME (INL (prop_imp p2 p3)) => p1 = p2 /\ p = p3
+      | _ => F)
+   | _ => F
+End
+
+Theorem valid_derivation_deriv_impe_eq:
+ !t l1 l2 p. map_ok t ==>
+  valid_derivation_deriv_impe_cake t l1 l2 p = 
+   valid_derivation_deriv_impe (to_fmap t) l1 l2 p
+Proof
+ rw [valid_derivation_deriv_impe_cake,valid_derivation_deriv_impe] \\
+ rw [lookup_thm]
+QED
+
+val res = translate valid_derivation_deriv_impe_cake;
+
+Definition valid_derivation_deriv_nege_cake:
+  valid_derivation_deriv_nege_cake t l1 l2 p =
+     case p of 
+     | prop_cont => 
+       (case lookup t (INL l1) of
+	| SOME (INL p1) =>
+	  (case lookup t (INL l2) of
+	   | SOME (INL (prop_neg p2)) => p1 = p2
+	   | _ => F)
+	| _ => F)
+     | _ => F
+End
+
+Theorem valid_derivation_deriv_nege_eq:
+ !t l1 l2 p. map_ok t ==>
+  valid_derivation_deriv_nege_cake t l1 l2 p = 
+   valid_derivation_deriv_nege (to_fmap t) l1 l2 p
+Proof
+ rw [valid_derivation_deriv_nege_cake,valid_derivation_deriv_nege] \\
+ rw [lookup_thm]
+QED
+
+val res = translate valid_derivation_deriv_nege_cake;
+
+Definition valid_derivation_deriv_conte_cake:
+ valid_derivation_deriv_conte_cake t l =
+   case lookup t (INL l) of
+   | SOME (INL prop_cont)  => T     
+   | _ => F
+End
+
+Theorem valid_derivation_deriv_conte_eq:
+ !t l p. map_ok t ==>
+  valid_derivation_deriv_conte_cake t l = 
+   valid_derivation_deriv_conte (to_fmap t) l
+Proof
+ rw [valid_derivation_deriv_conte_cake,valid_derivation_deriv_conte] \\
+ rw [lookup_thm]
+QED
+
+val res = translate valid_derivation_deriv_conte_cake;
+
+Definition valid_derivation_deriv_negnegi_cake:
+  valid_derivation_deriv_negnegi_cake t l p =
+    case p of
+    | prop_neg (prop_neg p1) => 
+      (case lookup t (INL l) of
+	| SOME (INL p2) => p1 = p2
+	| _ => F)
+    | _ => F
+End
+
+Theorem valid_derivation_deriv_negnegi_eq:
+ !t l p. map_ok t ==>
+  valid_derivation_deriv_negnegi_cake t l p = 
+   valid_derivation_deriv_negnegi (to_fmap t) l p
+Proof
+ rw [valid_derivation_deriv_negnegi_cake,valid_derivation_deriv_negnegi] \\
+ rw [lookup_thm]
+QED
+
+val res = translate valid_derivation_deriv_negnegi_cake;
+
+Definition valid_derivation_deriv_negnege_cake:
+ valid_derivation_deriv_negnege_cake t l p =
+  case lookup t (INL l) of
+  | SOME (INL (prop_neg (prop_neg p'))) => p' = p
+  | _ => F
+End
+
+Theorem valid_derivation_deriv_negnege_eq:
+ !t l p. map_ok t ==>
+  valid_derivation_deriv_negnege_cake t l p =   
+   valid_derivation_deriv_negnege (to_fmap t) l p   
+Proof
+ rw [valid_derivation_deriv_negnege_cake,valid_derivation_deriv_negnege] \\
+ rw [lookup_thm]
+QED
+
+val res = translate valid_derivation_deriv_negnege_cake;
+
+Definition valid_derivation_deriv_mt_cake:
+  valid_derivation_deriv_mt_cake t l1 l2 p =
+    case p of
+    | prop_neg p' =>
+      (case lookup t (INL l1) of
+       | SOME (INL (prop_imp p1 p2)) =>
+	 if p' = p1 then
+	     (case lookup t (INL l2) of
+	     | SOME (INL (prop_neg p3)) => p2 = p3
+	     | _ => F)
+	 else F
+       | _ => F)
+    | _ => F
+End
+
+Theorem valid_derivation_deriv_mt_eq:
+ !t l1 l2 p. map_ok t ==>
+  valid_derivation_deriv_mt_cake t l1 l2 p = 
+   valid_derivation_deriv_mt (to_fmap t) l1 l2 p
+Proof
+ rw [valid_derivation_deriv_mt_cake,valid_derivation_deriv_mt] \\
+ rw [lookup_thm]
+QED
+
+val res = translate valid_derivation_deriv_mt_cake;
+
+Definition valid_derivation_deriv_impi_cake:
+  valid_derivation_deriv_impi_cake t l1 l2 p =
+    case p of
+    | prop_imp p1 p2 => 
+      (case lookup t (INR (l1, l2)) of
+      | SOME (INR (p3, p4)) => p1 = p3 /\ p2 = p4
+      | _ => F)
+    | _ => F
+End
+
+Theorem valid_derivation_deriv_impi_eq:
+ !t l1 l2 p. map_ok t ==>
+  valid_derivation_deriv_impi_cake t l1 l2 p = 
+   valid_derivation_deriv_impi (to_fmap t) l1 l2 p
+Proof
+ rw [valid_derivation_deriv_impi_cake,valid_derivation_deriv_impi] \\
+ rw [lookup_thm]
+QED
+
+val res = translate valid_derivation_deriv_impi_cake;
+
+Definition valid_derivation_deriv_negi_cake:
+ valid_derivation_deriv_negi_cake t l1 l2 p =
+   case p of
+   | prop_neg p1 => 
+     (case lookup t (INR (l1,l2)) of
+      | SOME (INR (p2,prop_cont)) => p1 = p2	
+      | _ => F)
+   | _ => F
+End
+
+Theorem valid_derivation_deriv_negi_eq:
+ !t l1 l2 p. map_ok t ==>
+  valid_derivation_deriv_negi_cake t l1 l2 p = 
+   valid_derivation_deriv_negi (to_fmap t) l1 l2 p
+Proof
+ rw [valid_derivation_deriv_negi_cake,valid_derivation_deriv_negi] \\
+ rw [lookup_thm]
+QED
+
+val res = translate valid_derivation_deriv_negi_cake;
+
+Definition valid_derivation_deriv_ore_cake:
+  valid_derivation_deriv_ore_cake t l1 l2 l3 l4 l5 p =
+    case lookup t (INL l1) of
+    | SOME (INL (prop_or p1 p2)) => 
+      (case lookup t (INR (l2, l3)) of
+       | SOME (INR (p3, p4)) => 
+	 if p1 = p3 /\ p = p4 then
+	     (case lookup t (INR (l4,l5)) of
+              | SOME (INR (p5, p6)) =>
+		p2 = p5 /\ p = p6
+	      | _ => F)
+	 else F	     
+       | _ => F)
+    | _ => F
+End
+
+Theorem valid_derivation_deriv_ore_eq:
+ !t l1 l2 l3 l4 l5 p. map_ok t ==>
+  valid_derivation_deriv_ore_cake t l1 l2 l3 l4 l5 p = 
+   valid_derivation_deriv_ore (to_fmap t) l1 l2 l3 l4 l5 p
+Proof
+ rw [valid_derivation_deriv_ore_cake,valid_derivation_deriv_ore] \\
+ rw [lookup_thm]
+QED
+
+val res = translate valid_derivation_deriv_ore_cake;
+
+Definition valid_derivation_deriv_pbc_cake:
+  valid_derivation_deriv_pbc_cake t l1 l2 p =
+   case lookup t (INR (l1,l2)) of
+   | SOME (INR (prop_neg p', prop_cont)) =>
+     p' = p
+   | _ => F
+End
+
+Theorem valid_derivation_deriv_pbc_eq:
+ !t l1 l2 p. map_ok t ==>
+  valid_derivation_deriv_pbc_cake t l1 l2 p = 
+   valid_derivation_deriv_pbc (to_fmap t) l1 l2 p
+Proof
+ rw [valid_derivation_deriv_pbc_cake,valid_derivation_deriv_pbc] \\
+ rw [lookup_thm]
+QED
+
+val res = translate valid_derivation_deriv_pbc_cake;
+
+Definition valid_derivation_deriv_cake:
+  valid_derivation_deriv_cake t pl p r =
+    case r of
+    | reason_assumption => F
+    | reason_justification j => 
+      case j of
+      | justification_premise =>  valid_derivation_deriv_premise_cake pl p
+      | justification_lem => valid_derivation_deriv_lem_cake p
+      | justification_copy l => valid_derivation_deriv_copy_cake t l p
+      | justification_andi l1 l2  => valid_derivation_deriv_andi_cake t l1 l2 p
+      | justification_ande1 l => valid_derivation_deriv_ande1_cake t l p
+      | justification_ande2 l => valid_derivation_deriv_ande2_cake t l p
+      | justification_ori1 l => valid_derivation_deriv_ori1_cake t l p
+      | justification_ori2 l => valid_derivation_deriv_ori2_cake t l p
+      | justification_impe l1 l2 => valid_derivation_deriv_impe_cake t l1 l2 p
+      | justification_nege l1 l2 => valid_derivation_deriv_nege_cake t l1 l2 p
+      | justification_conte l => valid_derivation_deriv_conte_cake t l
+      | justification_negnegi l => valid_derivation_deriv_negnegi_cake t l p
+      | justification_negnege l => valid_derivation_deriv_negnege_cake t l p
+      | justification_mt l1 l2 => valid_derivation_deriv_mt_cake t l1 l2 p
+      | justification_impi l1 l2 => valid_derivation_deriv_impi_cake t l1 l2 p
+      | justification_negi l1 l2 => valid_derivation_deriv_negi_cake t l1 l2 p
+      | justification_ore l1 l2 l3 l4 l5 => valid_derivation_deriv_ore_cake t l1 l2 l3 l4 l5 p
+      | justification_pbc l1 l2 => valid_derivation_deriv_pbc_cake t l1 l2 p
+End
+
+Theorem valid_derivation_deriv_eq:
+  !t pl l p r. map_ok t ==> 
+  valid_derivation_deriv_cake t pl p r = valid_derivation_deriv (to_fmap t) pl p r
+Proof
+  rw [valid_derivation_deriv_cake,valid_derivation_deriv] \\
+  rw [valid_derivation_deriv_premise_eq] \\
+  rw [valid_derivation_deriv_lem_eq] \\
+  rw [valid_derivation_deriv_copy_eq] \\
+  rw [valid_derivation_deriv_andi_eq] \\
+  rw [valid_derivation_deriv_ande1_eq] \\
+  rw [valid_derivation_deriv_ande2_eq] \\
+  rw [valid_derivation_deriv_ori1_eq] \\
+  rw [valid_derivation_deriv_ori2_eq] \\
+  rw [valid_derivation_deriv_impe_eq] \\
+  rw [valid_derivation_deriv_nege_eq] \\
+  rw [valid_derivation_deriv_conte_eq] \\
+  rw [valid_derivation_deriv_negnegi_eq] \\
+  rw [valid_derivation_deriv_negnege_eq] \\
+  rw [valid_derivation_deriv_mt_eq] \\
+  rw [valid_derivation_deriv_impi_eq] \\
+  rw [valid_derivation_deriv_negi_eq] \\
+  rw [valid_derivation_deriv_ore_eq] \\
+  rw [valid_derivation_deriv_pbc_eq] \\
+  Cases_on `r` \\ rw [] \\ Cases_on `j` \\ rw []
+QED
+
+val res = translate valid_derivation_deriv_cake;
+
 (*
 fun get_current_prog() =
 let
@@ -79,8 +444,6 @@ val _ = astPP.enable_astPP();
 
 val _ = print_term (get_current_prog());
 *)
-
-val _ = ml_prog_update close_local_block;
 
 val _ = ml_prog_update (close_module NONE);
 
